6.2345

Chapter6.v
@@ -152,3 +152,377 @@ Eval compute in (mypred_final two_gt0).
 (* ================================================================================ *)
 (** * 6.2 - Decidable Proposition Types *)
 
+(* ================================================================================ *)
+(** **            Q: Define [eq_nat_deciable : {n = m} + {n <> m} *)
+
+
+Definition eq_nat_decidable_raw : forall n m : nat, {n = m} + {n <> m}.
+  refine(
+    fix f (n m : nat) :=
+    match n, m with
+    | O, O => left (eq_refl O)
+    | S n', S m' => (match f n' m' with
+      | left _ => left _
+      | right _ => right _
+      end
+    )
+    | _, _ => right _
+    end);
+
+    try (intro Hcontra; discriminate || congruence).
+
+    try (match goal with
+    | [ H : n' = m' |- _] => rewrite H
+    end; reflexivity).
+
+Defined.
+
+Eval compute in eq_nat_decidable_raw 2 2.
+Eval compute in eq_nat_decidable_raw 2 3.
+
+(* ================================================================================ *)
+(** **            Q: v2 with [Yes]/[No]/[Reduce] notation *)
+
+Notation "'Yes'" := (left _ _).
+Notation "'No'" := (right _ _).
+Notation "'Reduce' x" := (if x then Yes else No) (at level 50).
+
+Definition eq_nat_decidable_v2 : forall n m : nat, {n = m} + {n <> m}.
+  refine(
+    fix f (n m : nat) :=
+    match n, m with
+    | O, O => Yes
+    | S n', S m' => Reduce (f n' m')
+    | _, _ => No
+    end)
+    ; crush.
+Defined.
+
+Eval compute in eq_nat_decidable_v2 2 2.
+Eval compute in eq_nat_decidable_v2 2 3.
+
+(* ================================================================================ *)
+(** **            Q: v3 in one line *)
+
+Definition eq_nat_decidable_v3 : forall n m : nat, {n = m} + {n <> m}.
+  decide equality.
+Defined.
+
+(* ================================================================================ *)
+(** **            Q: Define [In_decidable] with and without Yes/No/Reduce notation. *)
+
+Notation "x || y" := (if x then Yes else Reduce y).
+
+Section In_dec.
+    Variable A : Set.
+    Variable A_eq_dec : forall x y : A, {x = y} + {x <> y}.
+
+    Definition In_dec_raw : forall (x : A) l, {In x l} + {~(In x l)}.
+      refine (
+        fix f (x : A) (l : list A) :=
+          match l with
+          | nil => No
+          | cons x' l' => (
+              match A_eq_dec x x' with
+(** Notation : [A_eq_dec x x'] *)
+              | left Heq => left _
+(** Notation : [||] *)
+              | right Hneq => (
+(** Notation : [Refine f x l'] *)
+                  match f x l' with
+                  | left _ => left _
+                  | right _ => right _
+                  end
+              )
+              end
+          )
+          end
+      ); crush.
+    Defined.
+
+    Definition In_dec : forall (x : A) l, {In x l} + {~(In x l)}.
+      refine (
+        fix f (x : A) (l : list A) :=
+          match l with
+          | nil => No
+          | cons x' l' => A_eq_dec x x' || f x l'
+          end); crush.
+    Defined.
+
+End In_dec.
+
+Eval compute in (In_dec_raw eq_nat_dec 2 (1 :: 2 :: nil)).
+Eval compute in (In_dec_raw eq_nat_dec 3 (1 :: 2 :: nil)).
+Eval compute in (In_dec_raw eq_nat_dec 2 (nil)).
+
+
+(* ================================================================================ *)
+(** * 6.3 - Partial Subset Types *)
+
+(* ================================================================================ *)
+(** **            Q: Define The [maybe] type *)
+
+Inductive maybe (A : Set) (P : A -> Prop) : Set :=
+| Unknown : maybe P
+(** Alternative : [| Found (x : A) (H : P x) : maybe P] *)
+| Found : forall x : A, P x -> maybe P
+.
+
+Notation "{{ x | P }}" := (maybe (fun x => P)).
+Notation "??" := (Unknown _).
+Notation "[| x |]" := (Found _ x _).
+
+(* ================================================================================ *)
+(** **            Q: v7 of [pred], using the [maybe] notation. *)
+
+Definition pred_v7 : forall n : nat, {{ m | S m = n }}.
+  refine (
+    fun n =>
+      match n with
+      | O => ??
+      | S n' => [| n' |]
+      end
+  ); trivial.
+Defined.
+
+Eval compute in (pred_v7 3).
+Eval compute in (pred_v7 1).
+Eval compute in (pred_v7 0).
+
+(* ================================================================================ *)
+(** **            Q: Why is the [maybe] type too loose for pred here ? *)
+
+(** The below dummy implementation is valid, i.e. the function type
+    allows such useless implementations. *)
+
+Definition pred_dummy : forall n : nat, {{ m | S m = n}}.
+  refine ( fun n => ?? ).
+Defined.
+
+(** For sure we want the type to enforce pred values that make sense *)
+
+(* ================================================================================ *)
+(** **            Q: v8 of [pred], refusing dummy implementations. *)
+
+Locate "_ + { _ }".
+Print sumor.
+
+Locate "[ _ ]".
+Print sig.
+Check exist.
+Notation "!!" := (inright _).
+Notation "[|| x ||]" := (inleft [x]).
+
+Definition pred_v8_raw : forall n : nat, {m : nat | S m = n} + {n = 0}.
+  refine( fun n =>
+    match n with
+    | O => inright (eq_refl 0)
+    | S n' => inleft (exist _ n' (eq_refl _ ))
+    end
+  ).
+Defined.
+
+Definition pred_v8 : forall n : nat, {m : nat | S m = n} + {n = 0}.
+  refine( fun n =>
+    match n with
+    | O => !!
+    | S n' => [|| n' ||]
+    end
+  ); trivial.
+Defined.
+
+Definition pred_dummy8 : forall n : nat, {m : nat | S m = n} + {n = 0}.
+  Fail refine( fun n => ?? ).
+Abort.
+
+Eval compute in (pred_v8 4).
+Eval compute in (pred_v8 1).
+Eval compute in (pred_v8 0).
+
+(* ================================================================================ *)
+(** * 6.4 - Monadic Notations *)
+
+(* ================================================================================ *)
+(** **            Q: Write a version of [double_pred] using [maybe]. *)
+
+Print maybe.
+
+Notation "x <-- e1 ; e2" := (match e1 with
+                           | Unknown _ => ??
+                           | Found _ x H => e2
+                           end)
+(right associativity, at level 60).
+
+Definition double_pred : forall n m : nat, {{ p | S (fst p) = n /\ S (snd p) = m}}.
+  refine(
+    fun n m =>
+    n' <-- pred_v7 n;
+    m' <-- pred_v7 m;
+    [| (n', m') |]); crush.
+Defined.
+
+
+(* ================================================================================ *)
+(** **            Q: Write a version of [double_pred] using [sumor]. *)
+
+Print sumor.
+Locate "!!". (* inright _ : sumor _ _ *)
+Locate "[|| x ||]". (* inleft (exist _ x _) : sumor *)
+Notation "x <--- e1 ; e2" :=
+( match e1 with
+| inright _ => !!
+| inleft (exist _ x _) => e2
+end)
+(right associativity, at level 60).
+
+Definition double_pred_sumor : forall n m : nat,
+  {p | S (fst p) = n /\ S (snd p) = m}  +  {n = 0 \/ m = 0}.
+  refine (
+    fun n m =>
+    n' <--- pred_v8 n;
+    m' <--- pred_v8 m;
+    [|| (n', m') ||]
+  );
+  try (unfold fst; unfold snd; split; assumption);
+  try (left; assumption);
+  try (right; assumption).
+Defined.
+
+
+(* ================================================================================ *)
+(** * 6.5 - A Type-Checking Example *)
+
+(** The idea here is to illustrate above techniques
+    on a certified type-checker for a language
+    with arithmetic and boolean expressions. *)
+
+Inductive exp : Set :=
+| E_Nat : nat -> exp
+| E_Plus : exp -> exp -> exp
+| E_Bool : bool -> exp
+| E_And : exp -> exp -> exp
+.
+
+Inductive typ : Set :=
+| T_Nat
+| T_Bool
+.
+
+Inductive hasType : exp -> typ -> Prop :=
+| HT_Nat : forall n : nat,
+    hasType (E_Nat n) T_Nat
+| HT_Plus : forall e1 e2 : exp,
+    hasType e1 T_Nat
+ -> hasType e2 T_Nat 
+ -> hasType (E_Plus e1 e2) T_Nat
+| HT_Bool : forall b : bool,
+    hasType (E_Bool b) T_Bool
+| HT_And : forall e1 e2 : exp,
+    hasType e1 T_Bool
+ -> hasType e2 T_Bool
+ -> hasType (E_And e1 e2) T_Bool
+.
+
+Definition eq_type_dec : forall t1 t2 : typ, {t1 = t2} + {t1 <> t2}.
+  decide equality.
+Defined.
+
+Notation "e1 ;; e2" := (if e1 then e2 else ??)
+(right associativity, at level 60).
+
+Locate "{{ _ | _ }}". (* maybe notation *)
+Print maybe.
+Locate "[| _  |]". (* maybe witness, for {{ t | P t }}, give [| t_witness |]*)
+Locate "??". (* maybe's Unknown *)
+
+
+Print hasType.
+
+Definition typeCheck : forall e : exp, {{ t | hasType e t }}.
+  Hint Constructors hasType.
+  refine( fix F (e : exp) : {{ t | hasType e t }} :=
+    match e return {{t | hasType e t}} with
+    | E_Nat _ => [| T_Nat |]
+    | E_Plus e1 e2 =>
+      t1 <-- F e1; (* returns ?? if e1 can't be typed *)
+      t2 <-- F e2; (* returns ?? if e1 can't be typed *) 
+      eq_type_dec t1 T_Nat;;
+      eq_type_dec t2 T_Nat;;
+
+      (*
+      H0 <-- eq_type_dec t1 T_Nat; (* returns ?? if it's the second ctor, i.e. [<>] *)
+      H2 <-- eq_type_dec t2 T_Nat; (* returns ?? if it's the second ctor, i.e. [<>] *)
+      *)
+      [| T_Nat |]
+    | E_Bool _ => [| T_Bool |]
+    | E_And e1 e2 =>
+      t1 <-- F e1;
+      t2 <-- F e2;
+      eq_type_dec t1 T_Bool;;
+      eq_type_dec t2 T_Bool;;
+      [| _ |]
+    end
+  );
+  try subst;
+  try constructor;
+  try assumption.
+Defined.
+
+Eval compute in typeCheck (E_Nat 0).
+Eval compute in typeCheck (E_Plus (E_Nat 0) (E_Nat 1)).
+Eval compute in typeCheck (E_Plus (E_Nat 0) (E_Bool false)).
+Eval compute in typeCheck (E_And (E_Bool true) (E_Bool false)).
+Eval compute in typeCheck (E_And (E_Bool true) (E_Nat 42)).
+
+
+Print maybe.
+Locate "??".
+Locate "[| _ |]".
+Locate "{{ _ | _ }}".
+
+Print sumor.
+Locate "!!".
+Locate "[|| _ ||]".
+Locate "_ + { _ }".
+
+Notation "e1 ;;; e2" := (if e1 then e2 else !!)
+(right associativity, at level 60).
+
+Lemma hasType_det : forall e t1, hasType e t1 ->
+  forall t2, hasType e t2 -> t1 = t2.
+Proof.
+    induction 1; inversion 1; reflexivity.
+Qed.
+
+Definition typeCheck' : forall e : exp, {t | hasType e t} + {forall t, ~ hasType e t}.
+  Hint Constructors hasType.
+  Hint Resolve hasType_det.
+  refine(
+    fix F (e : exp) :=
+      match e return {t | hasType e t} + {forall t, ~ hasType e t} with
+      | E_Nat _ => [|| T_Nat ||]
+      | E_Plus e1 e2 =>
+        t1 <--- F e1;
+        t2 <--- F e2;
+        eq_type_dec t1 T_Nat;;;
+        eq_type_dec t2 T_Nat;;;
+        [|| T_Nat ||]
+      | E_Bool _ => [|| T_Bool ||]
+      | E_And e1 e2 =>
+        t1 <--- F e1;
+        t2 <--- F e2;
+        eq_type_dec t1 T_Bool;;;
+        eq_type_dec t2 T_Bool;;;
+        [|| T_Bool ||]
+      end
+  )
+  ; clear F; crush' tt hasType; eauto.
+Defined.
+
+Eval compute in typeCheck' (E_Nat 0).
+Eval compute in typeCheck' (E_Plus (E_Nat 1) (E_Nat 2)).
+Eval compute in typeCheck' (E_Plus (E_Nat 1) (E_Bool true)).
+
+Eval compute in typeCheck' (E_Bool true).
+Eval compute in typeCheck' (E_And (E_Bool false) (E_Bool true)).
+Eval compute in typeCheck' (E_And (E_Nat 1) (E_Bool true)).
